negation rules 18 --> 9

negations/nrefinement.v
@@ -11,227 +11,9 @@ Require Import Coq.Logic.Classical_Pred_Type Coq.Logic.ClassicalFacts Coq.Logic.
 
 (* Require dpdgraph.dpdgraph. *)
 
-Lemma act_eq_neq: forall w w', (act_eq w w' -> False) -> act_neq w w'.
-Proof. intros.
-       unfold act_eq, act_neq in *.
-       apply not_all_ex_not in H.
-       destruct H as (a, H).
-       exists a.
-       unfold iff in H.
-       apply not_and_or in H.
-       destruct H as [H | H].
-       apply imply_to_and in H.
-       left. easy.
-       apply imply_to_and in H.
-       right. easy.
-Qed.
-
-Lemma actNeq: forall w1 w2, act_neq w1 w2 -> w1 ~< w2 -> False.
-Proof. intros.
-       unfold act_neq in H.
-       destruct H as ((q,ac), [ (Ha, Hb) | (Ha, Hb)]).
-       - case_eq ac; intros.
-         + subst. apply Hb.
-           punfold H0. inversion H0.
-           subst. apply mem_ext in H2.
-           case_eq (eqb p q); intros.
-           ++ rewrite eqb_eq in H3. subst.
-              rewrite h1. apply eq0. right. 
-              rewrite(coseq_eq(act (q & [(l, s', w')]))). unfold coseq_id.
-              simpl.
-              apply CoInSplit1 with (y := (q, rcv)) (ys:= (act w')).
-              simpl. easy. easy.
-           ++ rewrite eqb_neq in H3.
-              unfold act_eq in H2.
-              rewrite(coseq_eq(act (p & [(l, s, w)]))) in Ha.
-              unfold coseq_id in Ha. simpl in Ha.
-              inversion Ha. subst. simpl in H4. inversion H4.
-              subst. easy.
-              subst. simpl in H4. inversion H4. subst.
-              apply H2 in H6.
-              rewrite h1 in H6.
-              rewrite h1.
-              apply eq0.
-              apply dsanew in H6.
-              destruct H6 as [H6 | H6].
-              * left. easy.
-              * right.
-                rewrite(coseq_eq(act (p & [(l, s', w')]))). unfold coseq_id.
-                simpl. 
-                apply CoInSplit2 with (y := (p, rcv)) (ys:= (act w')). simpl. easy. easy. easy.
-         + subst. apply mem_ext in H2.
-           rewrite h0. apply eq0.
-           rewrite(coseq_eq(act (p ! [(l, s, w)]))) in Ha. unfold coseq_id in Ha.
-           simpl in Ha. inversion Ha.
-           subst. easy.
-           subst.
-           simpl in H3. inversion H3. subst.
-           unfold act_eq in H2.
-           apply H2 in H5.
-           rewrite h0 in H5. apply dsanew in H5.
-           destruct H5 as [H5 | H5].
-           left. easy.
-           right.
-           apply CoInSplit2 with (y := (p, snd)) (ys:= (act w')). simpl. easy. easy. easy.
-         + subst. rewrite(coseq_eq(act (end))) in Ha.
-           unfold coseq_id in Ha. simpl in Ha.
-           inversion Ha. subst. easy. subst. easy.
-           apply refinementR_mon.
-       - subst. apply Hb.
-         punfold H0. inversion H0.
-         subst. apply mem_ext in H2.
-         rewrite(coseq_eq(act (p & [(l, s, w)]))) in Ha.
-         unfold coseq_id in Ha. simpl in Ha. 
-         inversion Ha. subst. simpl in H3. easy.
-         subst. simpl in H3. inversion H3. subst.
-         apply H2 in H5.
-         rewrite h1 in H5.
-         apply dsbnew in H5.
-         rewrite h1.
-         apply eq0.
-         destruct H5 as [H5 | H5].
-         left. easy.
-         right.
-         apply CoInSplit2 with (y := (p, rcv)) (ys:= (act w')). simpl. easy. easy. easy.
-         subst. apply mem_ext in H2.
-         case_eq (eqb p q); intros.
-         ++ rewrite eqb_eq in H3. subst.
-            rewrite h0. apply eq0. right.
-            rewrite(coseq_eq(act (q ! [(l, s', w')]))). unfold coseq_id. simpl.
-            apply CoInSplit1 with (y := (q, snd)) (ys:= (act w')). easy. easy.
-         ++ rewrite eqb_neq in H3.
-            unfold act_eq in H2.
-            rewrite(coseq_eq(act (p ! [(l, s, w)]))) in Ha.
-            unfold coseq_id in Ha. simpl in Ha.
-            inversion Ha. subst. simpl in H4. inversion H4.
-            subst. easy.
-            subst. simpl in H4. inversion H4. subst.
-            apply H2 in H6.
-            rewrite h0 in H6.
-            rewrite h0.
-            apply eq0.
-            apply dsbnew in H6.
-            destruct H6 as [H6 | H6].
-            left. easy.
-            right.
-            rewrite(coseq_eq(act (p ! [(l, s', w')]))). unfold coseq_id. simpl.
-            apply CoInSplit2 with (y := (p, snd)) (ys:= (act w')). simpl. easy. easy. easy.
-         ++ subst. rewrite(coseq_eq(act (end))) in Ha.
-             unfold coseq_id in Ha. simpl in Ha.
-             inversion Ha. subst. easy. subst. easy.
-             apply refinementR_mon.
-
-       - case_eq ac; intros.
-         + subst. apply Hb.
-           punfold H0. inversion H0.
-           subst. apply mem_ext in H2.
-           case_eq (eqb p q); intros.
-           ++ rewrite eqb_eq in H3. subst.
-              rewrite(coseq_eq(act (q & [(l, s, w)]))). unfold coseq_id. simpl.
-              apply CoInSplit1 with (y := (q, rcv)) (ys:= (act w)). easy. easy.
-           ++ rewrite eqb_neq in H3.
-              unfold act_eq in H2.
-              rewrite h1 in Ha.
-              apply dsanew in Ha.
-              assert(In (q, rcv) (actAn p a n) \/ coseqIn (q, rcv) (act w')).
-              { destruct Ha. left. easy.
-                right.
-                inversion H4. subst. simpl in H5.
-                inversion H5. subst. easy.
-                inversion H5.
-                subst. easy.
-              }
-              apply eq0Anew in H4.
-              rewrite h1 in H2.
-              apply H2 in H4.
-              rewrite(coseq_eq(act (p & [(l, s, w)]))). unfold coseq_id. simpl.
-              apply CoInSplit2 with (y := (p, rcv)) (ys:= (act w)). simpl. easy.
-              unfold not. intro Hx. apply H3.
-              inversion Hx. easy. easy.
-              subst.
-              unfold act_eq in H2.
-              apply mem_ext in H2.
-              rewrite h0 in Ha.
-              apply dsanew in Ha.
-              assert(In (q, rcv) (actBn p b n) \/ coseqIn (q, rcv) (act w')).
-              { destruct Ha. left. easy.
-                right.
-                inversion H3. subst. simpl in H4. easy.
-                subst. simpl in H4. inversion H4. subst. easy.
-              }
-              apply eq0Anew in H3.
-              unfold act_eq in H2.
-              rewrite h0 in H2.
-              apply H2 in H3.
-              rewrite(coseq_eq(act (p ! [(l, s, w)]))). unfold coseq_id. simpl.
-              apply CoInSplit2 with (y := (p, snd)) (ys:= (act w)). simpl. easy. easy. easy.
-              subst. rewrite(coseq_eq(act (end))) in Ha.
-              unfold coseq_id in Ha. simpl in Ha.
-              inversion Ha. subst. easy. subst. easy.
-              apply refinementR_mon.
-         + subst.
-           apply Hb.
-           punfold H0. inversion H0.
-           subst. apply mem_ext in H2.
-           unfold act_eq in H2.
-           rewrite h1 in H2.
-           rewrite h1 in Ha.
-           apply dsbnew in Ha.
-           assert(In (q, snd) (actAn p a n) \/ coseqIn (q, snd) (act w')).
-           { destruct Ha. left. easy.
-             right.
-                inversion H3. subst. simpl in H4. easy.
-                subst. simpl in H4. inversion H4. subst. easy.
-           }
-           apply eq0Anew in H3.
-           apply H2 in H3.
-           rewrite(coseq_eq(act (p & [(l, s, w)]))). unfold coseq_id. simpl.
-           apply CoInSplit2 with (y := (p, rcv)) (ys:= (act w)). simpl. easy. easy. easy.
-         + subst.
-         case_eq (eqb p q); intros.
-         ++ rewrite eqb_eq in H3. subst.
-            rewrite(coseq_eq(act (q ! [(l, s, w)]))). unfold coseq_id. simpl.
-            apply CoInSplit1 with (y := (q, snd)) (ys:= (act w)). simpl. easy. easy.
-         ++ rewrite eqb_neq in H3.
-            unfold act_eq in H2.
-            apply mem_ext in H2.
-            rewrite h0 in Ha.
-            apply dsbnew in Ha.
-            assert(In (q, snd) (actBn p b n) \/ coseqIn (q, snd) (act w')).
-            { destruct Ha.
-              left. easy.
-              right.
-                inversion H4. subst. simpl in H5.
-                inversion H5. subst. easy.
-                inversion H5.
-                subst. easy.
-            }
-            apply eq0Anew in H4.
-            unfold act_eq in H2.
-            rewrite h0 in H2.
-            apply H2 in H4.
-            rewrite(coseq_eq(act (p ! [(l, s, w)]))). unfold coseq_id. simpl.
-            apply CoInSplit2 with (y := (p, snd)) (ys:= (act w)). simpl. easy.
-            intro Hx. apply H3. inversion Hx. easy. easy.
-            subst. rewrite(coseq_eq(act (end))) in Ha.
-            unfold coseq_id in Ha. simpl in Ha.
-            inversion Ha. subst. easy. subst. easy.
-            apply refinementR_mon.
-Qed.
-
 Inductive nRefinementN: siso -> siso -> Prop :=
-  | n_outN  : forall w w' p b l s P, 
-              (coseqIn (p,snd) (act (@und w')) -> False) -> 
-              nRefinementN (mk_siso (merge_bp_cont p b (st_send p [(l,s,(@und w))])) P) w'
-   | n_inpN  : forall w w' p c l s P, 
-              (coseqIn (p,rcv) (act (@und w')) -> False) -> 
-              nRefinementN (mk_siso (merge_cp_cont p c (st_receive p [(l,s,(@und w))])) P) w'
-  | n_out_rN: forall w w' p b l s P, 
-              (coseqIn (p,snd) (act (@und w)) -> False) -> 
-              nRefinementN w (mk_siso (merge_bp_cont p b (st_send p [(l,s,(@und w'))])) P)
-  | n_inp_rN: forall w w' p c l s P,
-              (coseqIn (p,rcv) (act (@und w)) -> False) -> 
-              nRefinementN w (mk_siso (merge_cp_cont p c (st_receive p [(l,s,(@und w'))])) P)
+  | n_actN  : forall w w' P Q,
+              act_neq w w' -> nRefinementN (mk_siso w P) (mk_siso w' Q)
   | n_a_lN  : forall w w' p l l' s s' a n P Q,
               l <> l' -> nRefinementN (mk_siso (st_receive p [(l,s,(@und w))]) P) 
                                       (mk_siso (merge_ap_contn p a (st_receive p [(l',s',(@und w'))]) n) Q)
@@ -261,6 +43,78 @@ Inductive nRefinementN: siso -> siso -> Prop :=
               nRefinementN w (mk_siso (merge_bp_contn p b (@und w') n) P) ->
               nRefinementN (mk_siso (st_send p [(l,s,(@und w))]) Q) 
                            (mk_siso (merge_bp_contn p b (st_send p [(l,s',(@und w'))]) n) R).
+
+Lemma n_outN: forall w w' p b l s P, 
+              (coseqIn (p,snd) (act (@und w')) -> False) -> 
+              nRefinementN (mk_siso (merge_bp_cont p b (st_send p [(l,s,(@und w))])) P) w'.
+Proof. intros.
+       destruct w' as (w', Q).
+       simpl in *.
+       simpl.
+       specialize(n_actN (merge_bp_cont p b (p ! [(l, s, und)])) w' P Q); intro Hneq.
+       apply Hneq.
+       unfold act_neq.
+       exists (p, snd).
+       left. split.
+       rewrite hm1. apply eq0.
+       right.
+       rewrite(coseq_eq(act (p ! [(l, s, und)]))). unfold coseq_id. simpl.
+       apply CoInSplit1 with (y := (p, snd)) (ys:= (act und)). simpl. easy. easy. easy.
+Qed.
+
+Lemma n_inpN: forall w w' p c l s P, 
+              (coseqIn (p,rcv) (act (@und w')) -> False) -> 
+              nRefinementN (mk_siso (merge_cp_cont p c (st_receive p [(l,s,(@und w))])) P) w'.
+Proof. intros.
+       destruct w' as (w', Q).
+       simpl in *.
+       simpl.
+       specialize(n_actN (merge_cp_cont p c (p & [(l, s, und)])) w' P Q); intro Hneq.
+       apply Hneq.
+       unfold act_neq.
+       exists (p, rcv).
+       left. split.
+       rewrite hm1c. apply eq0.
+       right.
+       rewrite(coseq_eq(act (p & [(l, s, und)]))). unfold coseq_id. simpl.
+       apply CoInSplit1 with (y := (p, rcv)) (ys:= (act und)). simpl. easy. easy. easy.
+Qed.
+
+Lemma n_out_rN: forall w w' p b l s P, 
+                (coseqIn (p,snd) (act (@und w)) -> False) -> 
+                nRefinementN w (mk_siso (merge_bp_cont p b (st_send p [(l,s,(@und w'))])) P).
+Proof. intros.
+       destruct w as (w, Q).
+       simpl in *.
+       simpl.
+       specialize(n_actN w (merge_bp_cont p b (p ! [(l, s, und)])) Q P); intro Hneq.
+       apply Hneq.
+       unfold act_neq.
+       exists (p, snd).
+       right. split.
+       rewrite hm1. apply eq0.
+       right.
+       rewrite(coseq_eq(act (p ! [(l, s, und)]))). unfold coseq_id. simpl.
+       apply CoInSplit1 with (y := (p, snd)) (ys:= (act und)). simpl. easy. easy. easy.
+Qed.
+
+Lemma n_inp_rN: forall w w' p c l s P,
+                (coseqIn (p,rcv) (act (@und w)) -> False) -> 
+                nRefinementN w (mk_siso (merge_cp_cont p c (st_receive p [(l,s,(@und w'))])) P).
+Proof. intros.
+       destruct w as (w, Q).
+       simpl in *.
+       simpl.
+       specialize(n_actN w (merge_cp_cont p c (p & [(l, s, und)])) Q P); intro Hneq.
+       apply Hneq.
+       unfold act_neq.
+       exists (p, rcv).
+       right. split.
+       rewrite hm1c. apply eq0.
+       right.
+       rewrite(coseq_eq(act (p & [(l, s, und)]))). unfold coseq_id. simpl.
+       apply CoInSplit1 with (y := (p, rcv)) (ys:= (act und)). simpl. easy. easy. easy.
+Qed.
 
 Lemma n_inp_lN: forall w w' p l l' s s' P Q,
                 l <> l' -> nRefinementN (mk_siso (st_receive p [(l,s,(@und w))]) P) 
